EFSMs using IMP

michael_formal/EFSM.thy
@@ -22,18 +22,28 @@ definition no_updates :: update_function where
   "no_updates _ r = r"
 declare no_updates_def [simp]
 
-definition possible_transitions :: "efsm \<Rightarrow> statename \<Rightarrow> registers \<Rightarrow> inputs \<Rightarrow> statename list" where
-  "possible_transitions e s r i = []"
+abbreviation is_possible_step :: "efsm \<Rightarrow> statename \<Rightarrow> statename \<Rightarrow> transition \<Rightarrow> registers \<Rightarrow> label \<Rightarrow> inputs \<Rightarrow> bool" where
+"is_possible_step e s s' t r l i \<equiv> (((Label t) = l) \<and> (find (\<lambda>x . x = t) (T e(s,s')) \<noteq> None) \<and> ((length i) = (Arity t)) \<and> ((Guard t) i r))"
 
-definition step :: "efsm \<Rightarrow> statename \<Rightarrow> registers \<Rightarrow> label \<Rightarrow> inputs \<Rightarrow> (outputs \<times> registers)" where
-  "step e s r l i = ([], <>)" (*For each step, return the outputs and updated registers *)
+abbreviation possible_steps :: "efsm \<Rightarrow> statename \<Rightarrow> registers \<Rightarrow> label \<Rightarrow> inputs \<Rightarrow> (statename * transition) list" where
+"possible_steps e s r l i \<equiv> [(s',t) . s' \<leftarrow> S e, t \<leftarrow> T e(s,s'), is_possible_step e s s' t r l i]"
+
+definition step :: "efsm \<Rightarrow> statename \<Rightarrow> registers \<Rightarrow> label \<Rightarrow> inputs \<Rightarrow> (statename \<times> outputs \<times> registers) option" where
+"step e s r l i \<equiv>
+  case (possible_steps e s r l i) of
+    [] \<Rightarrow> None |
+    [(s',t)] \<Rightarrow> Some (s', (apply_outputs t i r), (apply_updates t i r)) |
+    _ \<Rightarrow> None"
+declare step_def [simp]
 
 primrec observe_trace :: "efsm \<Rightarrow> statename \<Rightarrow> registers \<Rightarrow> trace \<Rightarrow> observation" where
   "observe_trace _ _ _ [] = []" |
-  "observe_trace e s r (h#t) = (outputs#(observe_trace e s updated t)) where
-  (outputs, updated) = step e s r label inputs
-  label = fst h
-  inputs = snd h"
+  "observe_trace e s r (h#t) = 
+    (case (step e s r (fst h) (snd h)) of
+      None \<Rightarrow> [] |
+      Some (s', outputs, updated) \<Rightarrow> (outputs#(observe_trace e s' updated t))
+    )"
+declare observe_trace_def [simp]
 
 
 
